# 풀이
- [STL 풀이](#c-stl-list-사용)
- [Doubly Linked List 구현 풀이](#circular-linked-list-구현)
------

## 풀이
```

```

### C++ STL List 사용
```c++
#include <iostream>
#include <list>
using namespace std;
typedef long long ll;

int	N, M;
int cnt;
int ans;
int main(void)
{
	ios::sync_with_stdio(false);
	cin.tie(NULL);

	list<int> List;
	list<int>::iterator it;
	list<int>::iterator match;

	cin >> N >> M;
	for (int idx = 1; idx <= N; ++idx)
		List.push_back(idx);
	it = List.begin();
	for (int idx = 1; idx <= M; ++idx)
	{
		int temp;
		cin >> temp;
		cnt = 0;
		for (; it != List.end();)
		{
			if (*it == temp)
				break ;
			else
			{
				++it;
				++cnt;
				if (it == List.end())
					it = List.begin();
			}
		}
		if (cnt <= List.size() / 2)
		{
			ans += cnt;
			it = List.erase(it);
			if (it == List.end())
				it = List.begin();
		}
		else
		{
			ans += (List.size() - cnt);
			it = List.erase(it);
			if (it == List.end())
				it = List.begin();
		}
	}
	cout << ans;
}
```

### Circular Linked List 구현
```c++
#include <iostream>
#include <stdlib.h>
using namespace std;
typedef long long ll;

typedef int LData;

typedef struct s_node
{
	LData data;
	struct s_node *next;
	struct s_node *prev;
} Node;

int	N, M;
int ans;
int main(void)
{
	ios::sync_with_stdio(false);
	cin.tie(NULL);

	cin >> N >> M;

	Node *tail = NULL;
	Node *head = NULL;
	for (int idx = 1; idx <= N; ++idx)
	{
		Node *newNode = (Node *)malloc(sizeof(Node));
		newNode->data = idx;
		if (tail == NULL)
		{
			tail = newNode;
			head = newNode;
		}
		else
		{
			newNode->prev = tail;
			tail->next = newNode;
			tail = newNode;
		}
	}
	tail->next = head;
	head->prev = tail;

	Node *curr = head;
	for (int idx = 1; idx <= M; ++idx)
	{
		int temp;
		cin >> temp;
		int cnt1 = 0;
		int cnt2 = 0;
		Node *right = curr;
		while (right->data != temp)
		{
			if (right->data == temp)
				break ;
			right = right->next;
			++cnt1;
		}
		Node *left = curr;
		while (left->data != temp)
		{
			if (left->data == temp)
				break ;
			left = left->prev;
			++cnt2;
		}
		if (cnt1 <= cnt2)
		{
			ans += cnt1;
			curr = right;
		}
		else
		{
			ans += cnt2;
			curr = left;
		}
		curr->next->prev = curr->prev;
		curr->prev->next = curr->next;
		curr = curr->next;
	}
	cout << ans;
}
```
